Port stack_remove make_init prerequisites word_loc/is_SOME_Word/read_mem/addresses

scripts/hol-probes/stack_remove_init_probeScript.sml
@@ -1,0 +1,18 @@
+load "preamble";
+load "stack_removeProofTheory";
+open bossLib;
+open HolKernel Parse;
+open preamble;
+open stack_removeProofTheory;
+
+fun print_eval label q =
+  (print label; print "="; print_term (rconc (EVAL q)); print "\n");
+
+val _ = print_eval "is_word_some" ``is_SOME_Word (SOME (Word (7w:8 word)))``;
+val _ = print_eval "is_word_loc" ``is_SOME_Word (SOME (Loc 1 2))``;
+val _ = print_eval "is_word_none" ``is_SOME_Word NONE``;
+val _ = print_eval "read_mem_len" ``LENGTH (read_mem (0w:8 word) (\x. Word x) 3)``;
+val _ = print_eval "read_mem_val" ``HD (read_mem (2w:8 word) (\x. Word (x + 1w)) 3)``;
+val _ = print_eval "in_addr_self" ``(0w:8 word) IN addresses (0w:8 word) 3``;
+val _ = print_eval "in_addr_step" ``(2w:8 word) IN addresses (0w:8 word) 3``;
+val _ = print_eval "in_addr_out" ``(5w:8 word) IN addresses (0w:8 word) 3``;
