Flapjack.lean
@@ -194,6 +194,7 @@ import Flapjack.Compiler.Backend.LabLang
 import Flapjack.Compiler.Backend.LabSem
 import Flapjack.Compiler.Backend.LabProps
 import Flapjack.Compiler.Backend.StackNames
+import Flapjack.Compiler.Backend.StackRemove
 import Flapjack.Compiler.Backend.StackAlloc
 import Flapjack.Compiler.Backend.WordToStack
 import Flapjack.RiscV.CakeAllocatorBitsBridge
